Added axioms 8.1 and 8.2, and continued with proving disquotation

fusion.ml
@@ -1175,7 +1175,7 @@ let rec type_subst i ty =
     let iet1 =  Comb(Comb(Const("isExprType",makeHolFunction (makeHolType "epsilon" []) (makeHolFunction (makeHolType "type" []) (makeHolType "bool" []))),tm1),matchType (makeHolFunction (type_of tm1) (type_of tm2))) in
     let iet2 =  Comb(Comb(Const("isExprType",makeHolFunction (makeHolType "epsilon" []) (makeHolFunction (makeHolType "type" []) (makeHolType "bool" []))),tm2),matchType (type_of tm2)) in
     let anticed = Comb(Comb(Const("/\\",makeHolFunction (makeHolType "bool" []) (makeHolFunction (makeHolType "bool" []) (makeHolType "bool" []))),iet1),iet2) in  
-    let conclud = safe_mk_eq (Eval(Comb(Comb(Const("app",makeHolFunction (makeHolType "epsilon" []) (makeHolFunction (makeHolType "epsilon" []) (makeHolType "epsilon" []))),tm1),tm2),(makeHolFunction (type_of tm1) (type_of tm2)))) (Comb(Eval(tm1,makeHolFunction (type_of tm1) (type_of tm2)),Eval(tm2,(type_of tm2)))) in
+    let conclud = safe_mk_eq (Eval(Comb(Comb(Const("app",makeHolFunction (makeHolType "epsilon" []) (makeHolFunction (makeHolType "epsilon" []) (makeHolType "epsilon" []))),tm1),tm2),((type_of tm1)))) (Comb(Eval(tm1,makeHolFunction (type_of tm1) (type_of tm2)),Eval(tm2,(type_of tm2)))) in
                            Sequent([], internal_make_imp anticed conclud)
 
   (*Axiom B11 (1)*)
